syntax

src/lang_handle.v
@@ -6,6 +6,16 @@ From iris.prelude Require Import options.
 Open Scope Z.
 
 (*|
+=====================================
+reghandle_lang
+=====================================
+
+This is the **handle** model of RegLang, kept alongside the primary annotation
+model [lang.v] for comparison: regions are first-class *values* [RegionV ρ],
+`region` binds an ordinary term variable that is substituted with such a handle,
+and `alloc er e` takes the region as an evaluated operand. The corresponding type
+system is [typing_handle.v]. 
+
 ===========
 Syntax
 ===========
@@ -19,22 +29,11 @@ Definition loc := Z.
 Definition region := Z.
 
 (*|
-A region annotation [rexpr]: a region variable [RVar x] (bound by `region`) or a
-concrete region name [RName ρ] (after substitution).
+Expressions are defined mutually recursively with values. As explained above, an
+expression is a value iff it uses the Val constructor, which makes defining
+reduction and substitution much simpler, but requires duplicating `Rec` and
+`Pair` to `val` as `RecV` and `PairV`.
 |*)
-Inductive rexpr :=
-  | RVar (x : string)
-  | RName (ρ : region).
-
-Global Instance rexpr_eq_dec : EqDecision rexpr.
-Proof. solve_decision. Defined.
-Global Instance rexpr_countable : Countable rexpr.
-Proof.
-  refine (inj_countable'
-            (λ r, match r with RVar x => inl x | RName ρ => inr ρ end)
-            (λ s, match s with inl x => RVar x | inr ρ => RName ρ end) _).
-  by intros [].
-Qed.
 
 Inductive expr :=
   (* Values *)
@@ -52,22 +51,30 @@ Inductive expr :=
   | InjR (e : expr)
   | Case (e0 : expr) (x1 : binder) (e1 : expr) (x2 : binder) (e2 : expr)
   (* Regions and references *)
-  | Alloc (r : rexpr) (e : expr)      
+  | Alloc (e1 : expr) (e2 : expr)     (* alloc INTO region [e1] the value [e2] *)
   | Load (e : expr)
   | Store (e1 : expr) (e2 : expr)
-  | LetRegion (x : binder) (e : expr)   
-  | EndRegion (ρ : region) (e : expr) 
+  | Region (x : binder) (e : expr)    (* region: x in e *)
+  | EndRegion (ρ : region) (e : expr) (* runtime only: deallocates [ρ] when [e] is a value *)
 with val :=
   | UnitV
   | PairV (v1 v2 : val)
   | InjLV (v : val)
   | InjRV (v : val)
   | RecV (f x : binder) (e : expr)
-  | RefV (ρ : region) (l : loc)     
+  | RegionV (ρ : region)              (* a region handle *)
+  | RefV (ρ : region) (l : loc)       (* a reference (ρ, ℓ) *)
 .
 
 Bind Scope expr_scope with expr.
 Bind Scope val_scope with val.
+
+(*|
+These define part of ectxi_language: we need a type for expressions, a type for
+values, and a way to go back and forth (where to_val is partial because only
+some expressions are values). Here the use of Val to identify all values makes
+this easy and non-recursive.
+|*)
 
 Notation of_val := Val (only parsing).
 
@@ -112,12 +119,12 @@ Proof.
        | Case e0 x1 e1 x2 e2, Case e0' x1' e1' x2' e2' =>
          cast_if_and5 (decide (e0 = e0')) (decide (x1 = x1')) (decide (e1 = e1'))
                       (decide (x2 = x2')) (decide (e2 = e2'))
-       | Alloc r e, Alloc r' e' =>
-         cast_if_and (decide (r = r')) (decide (e = e'))
+       | Alloc e1 e2, Alloc e1' e2' =>
+         cast_if_and (decide (e1 = e1')) (decide (e2 = e2'))
        | Load e, Load e' => cast_if (decide (e = e'))
        | Store e1 e2, Store e1' e2' =>
          cast_if_and (decide (e1 = e1')) (decide (e2 = e2'))
-       | LetRegion x e, LetRegion x' e' =>
+       | Region x e, Region x' e' =>
          cast_if_and (decide (x = x')) (decide (e = e'))
        | EndRegion ρ e, EndRegion ρ' e' =>
          cast_if_and (decide (ρ = ρ')) (decide (e = e'))
@@ -132,6 +139,7 @@ Proof.
        | InjRV v, InjRV v' => cast_if (decide (v = v'))
        | RecV f x e, RecV f' x' e' =>
          cast_if_and3 (decide (f = f')) (decide (x = x')) (decide (e = e'))
+       | RegionV ρ, RegionV ρ' => cast_if (decide (ρ = ρ'))
        | RefV ρ l, RefV ρ' l' =>
          cast_if_and (decide (ρ = ρ')) (decide (l = l'))
        | _, _ => right _
@@ -140,15 +148,14 @@ Defined.
 Global Instance expr_eq_dec' : EqDecision expr := expr_eq_dec.
 Global Instance val_eq_dec' : EqDecision val := val_eq_dec.
 
-
 Global Instance expr_countable : Countable expr.
 Proof.
  set (enc :=
    fix go e :=
      match e with
      | Val v => GenNode 0 [gov v]
-     | Var x => GenLeaf (inl (inl (inl x)))
-     | Rec f x e => GenNode 1 [GenLeaf (inl (inl (inr f))); GenLeaf (inl (inl (inr x))); go e]
+     | Var x => GenLeaf (inl (inl x))
+     | Rec f x e => GenNode 1 [GenLeaf (inl (inr f)); GenLeaf (inl (inr x)); go e]
      | App e1 e2 => GenNode 2 [go e1; go e2]
      | Pair e1 e2 => GenNode 3 [go e1; go e2]
      | Fst e => GenNode 4 [go e]
@@ -156,12 +163,12 @@ Proof.
      | InjL e => GenNode 6 [go e]
      | InjR e => GenNode 7 [go e]
      | Case e0 x1 e1 x2 e2 =>
-        GenNode 8 [go e0; GenLeaf (inl (inl (inr x1))); go e1; GenLeaf (inl (inl (inr x2))); go e2]
-     | Alloc r e => GenNode 9 [GenLeaf (inr r); go e]
+        GenNode 8 [go e0; GenLeaf (inl (inr x1)); go e1; GenLeaf (inl (inr x2)); go e2]
+     | Alloc e1 e2 => GenNode 9 [go e1; go e2]
      | Load e => GenNode 10 [go e]
      | Store e1 e2 => GenNode 11 [go e1; go e2]
-     | LetRegion x e => GenNode 12 [GenLeaf (inl (inl (inr x))); go e]
-     | EndRegion ρ e => GenNode 13 [GenLeaf (inl (inr (inl ρ))); go e]
+     | Region x e => GenNode 12 [GenLeaf (inl (inr x)); go e]
+     | EndRegion ρ e => GenNode 13 [GenLeaf (inr (inl ρ)); go e]
      end
    with gov v :=
      match v with
@@ -170,29 +177,30 @@ Proof.
      | InjLV v => GenNode 2 [gov v]
      | InjRV v => GenNode 3 [gov v]
      | RecV f x e =>
-        GenNode 4 [GenLeaf (inl (inl (inr f))); GenLeaf (inl (inl (inr x))); go e]
-     | RefV ρ l => GenNode 5 [GenLeaf (inl (inr (inl ρ))); GenLeaf (inl (inr (inr l)))]
+        GenNode 4 [GenLeaf (inl (inr f)); GenLeaf (inl (inr x)); go e]
+     | RegionV ρ => GenNode 5 [GenLeaf (inr (inl ρ))]
+     | RefV ρ l => GenNode 6 [GenLeaf (inr (inl ρ)); GenLeaf (inr (inr l))]
      end
    for go).
  set (dec :=
    fix go e :=
      match e with
      | GenNode 0 [v] => Val (gov v)
-     | GenLeaf (inl (inl (inl x))) => Var x
-     | GenNode 1 [GenLeaf (inl (inl (inr f))); GenLeaf (inl (inl (inr x))); e] => Rec f x (go e)
+     | GenLeaf (inl (inl x)) => Var x
+     | GenNode 1 [GenLeaf (inl (inr f)); GenLeaf (inl (inr x)); e] => Rec f x (go e)
      | GenNode 2 [e1; e2] => App (go e1) (go e2)
      | GenNode 3 [e1; e2] => Pair (go e1) (go e2)
      | GenNode 4 [e] => Fst (go e)
      | GenNode 5 [e] => Snd (go e)
      | GenNode 6 [e] => InjL (go e)
      | GenNode 7 [e] => InjR (go e)
-     | GenNode 8 [e0; GenLeaf (inl (inl (inr x1))); e1; GenLeaf (inl (inl (inr x2))); e2] =>
+     | GenNode 8 [e0; GenLeaf (inl (inr x1)); e1; GenLeaf (inl (inr x2)); e2] =>
         Case (go e0) x1 (go e1) x2 (go e2)
-     | GenNode 9 [GenLeaf (inr r); e] => Alloc r (go e)
+     | GenNode 9 [e1; e2] => Alloc (go e1) (go e2)
      | GenNode 10 [e] => Load (go e)
      | GenNode 11 [e1; e2] => Store (go e1) (go e2)
-     | GenNode 12 [GenLeaf (inl (inl (inr x))); e] => LetRegion x (go e)
-     | GenNode 13 [GenLeaf (inl (inr (inl ρ))); e] => EndRegion ρ (go e)
+     | GenNode 12 [GenLeaf (inl (inr x)); e] => Region x (go e)
+     | GenNode 13 [GenLeaf (inr (inl ρ)); e] => EndRegion ρ (go e)
      | _ => Val UnitV (* dummy *)
      end
    with gov v :=
@@ -201,8 +209,9 @@ Proof.
      | GenNode 1 [v1; v2] => PairV (gov v1) (gov v2)
      | GenNode 2 [v] => InjLV (gov v)
      | GenNode 3 [v] => InjRV (gov v)
-     | GenNode 4 [GenLeaf (inl (inl (inr f))); GenLeaf (inl (inl (inr x))); e] => RecV f x (go e)
-     | GenNode 5 [GenLeaf (inl (inr (inl ρ))); GenLeaf (inl (inr (inr l)))] => RefV ρ l
+     | GenNode 4 [GenLeaf (inl (inr f)); GenLeaf (inl (inr x)); e] => RecV f x (go e)
+     | GenNode 5 [GenLeaf (inr (inl ρ))] => RegionV ρ
+     | GenNode 6 [GenLeaf (inr (inl ρ)); GenLeaf (inr (inr l))] => RefV ρ l
      | _ => UnitV (* dummy *)
      end
    for go).
@@ -215,11 +224,13 @@ Qed.
 Global Instance val_countable : Countable val.
 Proof. refine (inj_countable of_val to_val _); auto using to_of_val. Qed.
 
+(** the language interface needs values and expressions to be inhabited *)
 Global Instance val_inhabited : Inhabited val := populate UnitV.
 Global Instance expr_inhabited : Inhabited expr := populate (Val UnitV).
 
-(**Evaluation Contexts *)
 
+
+(** Evaluation contexts *)
 Inductive ectx_item :=
   | AppLCtx (v2 : val)
   | AppRCtx (e1 : expr)
@@ -230,7 +241,8 @@ Inductive ectx_item :=
   | InjLCtx
   | InjRCtx
   | CaseCtx (x1 : binder) (e1 : expr) (x2 : binder) (e2 : expr)
-  | AllocCtx (r : rexpr)
+  | AllocLCtx (v2 : val)
+  | AllocRCtx (e1 : expr)
   | LoadCtx
   | StoreLCtx (v2 : val)
   | StoreRCtx (e1 : expr)
@@ -248,12 +260,19 @@ Definition fill_item (Ki : ectx_item) (e : expr) : expr :=
   | InjLCtx => InjL e
   | InjRCtx => InjR e
   | CaseCtx x1 e1 x2 e2 => Case e x1 e1 x2 e2
-  | AllocCtx r => Alloc r e
+  | AllocLCtx v2 => Alloc e (of_val v2)
+  | AllocRCtx e1 => Alloc e1 e
   | LoadCtx => Load e
   | StoreLCtx v2 => Store e (of_val v2)
   | StoreRCtx e1 => Store e1 e
   | EndRegionCtx ρ => EndRegion ρ e
   end.
+
+
+(*|
+We have to prove a few properties that show `fill_item` and `base_step` is
+reasonable for `ectxi_language`.
+|*)
 
 Global Instance fill_item_inj Ki : Inj (=) (=) (fill_item Ki).
 Proof. destruct Ki; intros ???; simplify_eq/=; auto with f_equal. Qed.
@@ -267,13 +286,9 @@ Lemma fill_item_no_val_inj Ki1 Ki2 e1 e2 :
   fill_item Ki1 e1 = fill_item Ki2 e2 → Ki1 = Ki2.
 Proof. destruct Ki1, Ki2; naive_solver eauto with f_equal. Qed.
 
-  
-(** Substitution **)
 
-(** We need two substitutions: subst, one for ordinary substitution that does not 
-  touch `LetRegion`, and subst_region, substitutions a name of a region. subst_region
-  does not stop at Rec/Case. **)
 
+(** Substitution *)
 Fixpoint subst (x : string) (v : val) (e : expr) : expr :=
   match e with
   | Val _ => e
@@ -290,51 +305,26 @@ Fixpoint subst (x : string) (v : val) (e : expr) : expr :=
     Case (subst x v e0)
          x1 (if decide (BNamed x ≠ x1) then subst x v e1 else e1)
          x2 (if decide (BNamed x ≠ x2) then subst x v e2 else e2)
-  | Alloc r e => Alloc r (subst x v e)
+  | Alloc e1 e2 => Alloc (subst x v e1) (subst x v e2)
   | Load e => Load (subst x v e)
   | Store e1 e2 => Store (subst x v e1) (subst x v e2)
-  | LetRegion y e => LetRegion y (subst x v e)   
+  | Region y e =>
+    Region y $ if decide (BNamed x ≠ y) then subst x v e else e
   | EndRegion ρ e => EndRegion ρ (subst x v e)
   end.
 
 Definition subst' (mx : binder) (v : val) : expr → expr :=
   match mx with BNamed x => subst x v | BAnon => id end.
 
-Definition subst_rexpr (x : string) (ρ : region) (r : rexpr) : rexpr :=
-  match r with
-  | RVar y => if decide (x = y) then RName ρ else RVar y
-  | RName ρ' => RName ρ'
-  end.
-
-Fixpoint subst_region (x : string) (ρ : region) (e : expr) : expr :=
-  match e with
-  | Val _ => e
-  | Var _ => e
-  | Rec f y e => Rec f y (subst_region x ρ e)
-  | App e1 e2 => App (subst_region x ρ e1) (subst_region x ρ e2)
-  | Pair e1 e2 => Pair (subst_region x ρ e1) (subst_region x ρ e2)
-  | Fst e => Fst (subst_region x ρ e)
-  | Snd e => Snd (subst_region x ρ e)
-  | InjL e => InjL (subst_region x ρ e)
-  | InjR e => InjR (subst_region x ρ e)
-  | Case e0 x1 e1 x2 e2 =>
-    Case (subst_region x ρ e0) x1 (subst_region x ρ e1) x2 (subst_region x ρ e2)
-  | Alloc r e => Alloc (subst_rexpr x ρ r) (subst_region x ρ e)
-  | Load e => Load (subst_region x ρ e)
-  | Store e1 e2 => Store (subst_region x ρ e1) (subst_region x ρ e2)
-  | LetRegion y e => LetRegion y $ if decide (BNamed x ≠ y) then subst_region x ρ e else e
-  | EndRegion ρ' e => EndRegion ρ' (subst_region x ρ e)
-  end.
-
-Definition subst_region' (mx : binder) (ρ : region) : expr → expr :=
-  match mx with BNamed x => subst_region x ρ | BAnon => id end.
-
 (*|
 ===========
 Semantics
 ===========
 
-*)
+State
+-----
+
+|*)
 
 Record state : Type := {
   heap : gmap (region * loc) val;
@@ -353,6 +343,8 @@ Definition state_upd_alive (f : gmap region bool → gmap region bool)
     (σ : state) : state :=
   {| heap := σ.(heap); alive := f σ.(alive) |}.
 Global Arguments state_upd_alive _ !_ /.
+
+
 
 Inductive observation :=.
 Lemma observations_empty (κs : list observation) : κs = [].
@@ -380,11 +372,11 @@ Inductive base_step :
     base_step (Case (Val $ InjLV v) x1 e1 x2 e2) σ [] (subst' x1 v e1) σ []
   | CaseRS v x1 e1 x2 e2 σ :
     base_step (Case (Val $ InjRV v) x1 e1 x2 e2) σ [] (subst' x2 v e2) σ []
-  | LetRegionS x e ρ σ :
+  | RegionS x e ρ σ :
     σ.(alive) !! ρ = None →
-    base_step (LetRegion x e) σ
+    base_step (Region x e) σ
               []
-              (EndRegion ρ (subst_region' x ρ e))
+              (EndRegion ρ (subst' x (RegionV ρ) e))
               (state_upd_alive <[ρ := true]> σ)
               []
   | EndRegionS ρ v σ :
@@ -396,7 +388,7 @@ Inductive base_step :
   | AllocS ρ l v σ :
     σ.(alive) !! ρ = Some true →
     σ.(heap) !! (ρ, l) = None →
-    base_step (Alloc (RName ρ) (Val v)) σ
+    base_step (Alloc (Val $ RegionV ρ) (Val v)) σ
               []
               (Val $ RefV ρ l) (state_upd_heap <[(ρ, l) := v]> σ)
               []
@@ -416,6 +408,7 @@ Inductive base_step :
               []
   .
 
+
 Lemma val_base_stuck e1 σ1 κ e2 σ2 efs : base_step e1 σ1 κ e2 σ2 efs → to_val e1 = None.
 Proof. destruct 1; naive_solver. Qed.
 
@@ -423,16 +416,17 @@ Lemma base_ctx_step_val Ki e σ1 κ e2 σ2 efs :
   base_step (fill_item Ki e) σ1 κ e2 σ2 efs → is_Some (to_val e).
 Proof. destruct Ki; inversion_clear 1; simplify_option_eq; eauto. Qed.
 
-(** Freshness lemmas for regions *)
+
+
 Lemma region_fresh σ : σ.(alive) !! fresh (dom σ.(alive)) = None.
 Proof. apply not_elem_of_dom, is_fresh. Qed.
 
-Lemma letregion_step_fresh x e σ :
+Lemma region_step_fresh x e σ :
   let ρ := fresh (dom σ.(alive)) in
-  base_step (LetRegion x e) σ []
-            (EndRegion ρ (subst_region' x ρ e))
+  base_step (Region x e) σ []
+            (EndRegion ρ (subst' x (RegionV ρ) e))
             (state_upd_alive <[ρ := true]> σ) [].
-Proof. apply LetRegionS, region_fresh. Qed.
+Proof. apply RegionS, region_fresh. Qed.
 
 Definition heap_locs (h : gmap (region * loc) val) : gset loc :=
   set_map snd (dom h).
@@ -444,33 +438,24 @@ Proof.
   apply (elem_of_map_2 (D:=gset loc) snd (dom h) (ρ, fresh (heap_locs h)) Hin).
 Qed.
 
-(** this theorem will be needed to show that allocation is never stuck when we
-prove a WP for it *)
 Lemma alloc_fresh ρ v σ :
   let l := fresh (heap_locs σ.(heap)) in
   σ.(alive) !! ρ = Some true →
-  base_step (Alloc (RName ρ) (Val v)) σ []
+  base_step (Alloc (Val $ RegionV ρ) (Val v)) σ []
             (Val $ RefV ρ l) (state_upd_heap <[(ρ, l) := v]> σ) [].
 Proof. intros l Halive. apply AllocS; [done|]. apply heap_loc_fresh. Qed.
 
-(*|
-This is really where we instantiate the language, by constructing a "mixin" and
-then using some canonical structures to build the full record.
 
-You can see that the mixin uses `fill_item` and `base_step` as the core of the
-semantics. It uses `of_val` and `to_val` to define a number of related notions
-like reducible and not-stuck and such.
-|*)
-
-Lemma reg_lang_mixin : EctxiLanguageMixin of_val to_val fill_item base_step.
+Lemma reghandle_lang_mixin : EctxiLanguageMixin of_val to_val fill_item base_step.
 Proof.
   split; apply _ || eauto using to_of_val, of_to_val, val_base_stuck,
     fill_item_val, fill_item_no_val_inj, base_ctx_step_val.
 Qed.
 
-Canonical Structure reg_ectxi_lang := EctxiLanguage reg_lang_mixin.
-Canonical Structure reg_ectx_lang := EctxLanguageOfEctxi reg_ectxi_lang.
-Canonical Structure reg_lang := LanguageOfEctx reg_ectx_lang.
+Canonical Structure reghandle_ectxi_lang := EctxiLanguage reghandle_lang_mixin.
+Canonical Structure reghandle_ectx_lang := EctxLanguageOfEctxi reghandle_ectxi_lang.
+Canonical Structure reghandle_lang := LanguageOfEctx reghandle_ectx_lang.
 
-Check (@step reg_lang).
-Eval compute in cfg reg_lang.
+
+Check (@step reghandle_lang).
+Eval compute in cfg reghandle_lang.
