src/typing_handle.v
@@ -1,0 +1,104 @@
+From iris_simp_lang Require Import lang_handle.
+From stdpp Require Import binders gmap.
+
+
+Inductive ty :=
+  | TUnit
+  | TProd (A B : ty)
+  | TSum (A B : ty)
+  | TArrow (A : ty) (σ : gset region) (B : ty)  
+  | TRef (ρ : region) (A : ty)                
+  | TRgn (ρ : region)                             (* region handle for ρ *)
+.
+
+Notation tctx := (gmap string ty).
+Notation eff  := (gset region).  
+
+
+Inductive typed : tctx → expr → ty → eff → Prop :=
+  | T_Var Γ x A :                                     (* RegTVar *)
+    Γ !! x = Some A →
+    typed Γ (Var x) A ∅
+  | T_Unit Γ :                                        (* RegTUnit *)
+    typed Γ (Val UnitV) TUnit ∅
+  | T_Pair Γ e1 e2 A B σ1 σ2 σ :                      (* RegTPair *)
+    typed Γ e1 A σ1 →
+    typed Γ e2 B σ2 →
+    σ = σ1 ∪ σ2 →
+    typed Γ (Pair e1 e2) (TProd A B) σ
+  | T_Fst Γ e A B σ :                                 (* RegTProj (i = 1) *)
+    typed Γ e (TProd A B) σ →
+    typed Γ (Fst e) A σ
+  | T_Snd Γ e A B σ :                                 (* RegTProj (i = 2) *)
+    typed Γ e (TProd A B) σ →
+    typed Γ (Snd e) B σ
+  | T_InjL Γ e A B σ :                                (* RegTInj (i = 1) *)
+    typed Γ e A σ →
+    typed Γ (InjL e) (TSum A B) σ
+  | T_InjR Γ e A B σ :                                (* RegTInj (i = 2) *)
+    typed Γ e B σ →
+    typed Γ (InjR e) (TSum A B) σ
+  | T_Case Γ e0 x1 e1 x2 e2 A B C σ0 σ1 σ2 σ :        (* RegTCase *)
+    typed Γ e0 (TSum A B) σ0 →
+    typed (binder_insert x1 A Γ) e1 C σ1 →
+    typed (binder_insert x2 B Γ) e2 C σ2 →
+    σ = σ0 ∪ σ1 ∪ σ2 →
+    typed Γ (Case e0 x1 e1 x2 e2) C σ
+  | T_Rec Γ f x e A B σf :                            (* RegTRec *)
+    typed (binder_insert f (TArrow A σf B) (binder_insert x A Γ)) e B σf →
+    typed Γ (Rec f x e) (TArrow A σf B) ∅
+  | T_App Γ e1 e2 A B σf σ1 σ2 σ :                    (* RegTApp *)
+    typed Γ e1 (TArrow A σf B) σ1 →
+    typed Γ e2 A σ2 →
+    σ = σ1 ∪ σ2 ∪ σf →
+    typed Γ (App e1 e2) B σ
+  | T_Alloc Γ er ev A ρ σr σv σ :                     (* RegTNew  *)
+    typed Γ er (TRgn ρ) σr →
+    typed Γ ev A σv →
+    σ = σr ∪ σv ∪ {[ρ]} →
+    typed Γ (Alloc er ev) (TRef ρ A) σ
+  | T_Load Γ e A ρ σe σ :                             (* RegTDeref *)
+    typed Γ e (TRef ρ A) σe →
+    σ = σe ∪ {[ρ]} →
+    typed Γ (Load e) A σ
+  | T_Store Γ e1 e2 A ρ σ1 σ2 σ :                     (* RegTAssign *)
+    typed Γ e1 (TRef ρ A) σ1 →
+    typed Γ e2 A σ2 →
+    σ = σ1 ∪ σ2 ∪ {[ρ]} →
+    typed Γ (Store e1 e2) TUnit σ
+  | T_Region Γ x e A σ :                              (* RegTMask  *)
+    (∀ ρ, typed (binder_insert x (TRgn ρ) Γ) e A (σ ∪ {[ρ]})) →
+    typed Γ (Region x e) A σ
+  | T_Sub Γ e A σ σ' :                                (* RegTSub *)
+    typed Γ e A σ →
+    σ ⊆ σ' →
+    typed Γ e A σ'
+.
+
+Open Scope string_scope.
+
+(** [(λ y. y) () : unit @ ∅]. *)
+Example app_id_typed :
+  typed ∅ (App (Rec BAnon "y" (Var "y")) (Val UnitV)) TUnit ∅.
+Proof.
+  eapply T_App.
+  - apply T_Rec. apply T_Var. rewrite /binder_insert /=. apply lookup_insert_eq.
+  - apply T_Unit.
+  - set_solver.
+Qed.
+
+(** [letregion r in (! (alloc_r ())) : unit @ ∅] *)
+Example region_alloc_load_typed :
+  typed ∅ (Region "x" (Load (Alloc (Var "x") (Val UnitV)))) TUnit ∅.
+Proof.
+  apply T_Region. intros ρ.
+  eapply T_Sub.
+  - eapply T_Load.
+    + eapply T_Alloc.
+      * apply T_Var. rewrite /binder_insert /=. apply lookup_insert_eq.
+      * apply T_Unit.
+      * reflexivity.
+    + reflexivity.
+  - set_solver.
+Qed.
+
